monoids

Monoid.v
@@ -39,7 +39,7 @@ Module MonoidFactory (MS : MonoidSpec).
 End MonoidFactory.
 
 (** Addition of Naturals. *)
-Module AdditionMonoidSpec <: MonoidSpec.
+Module AddMonoidSpec <: MonoidSpec.
 
   Definition A : Type := nat.
 
@@ -47,12 +47,122 @@ Module AdditionMonoidSpec <: MonoidSpec.
 
   Definition mappend : nat -> nat -> nat := add.
 
-  Lemma mempty_app_l : forall (a : A), 0 + a = a.
+  Lemma mempty_app_l : forall (a : nat), 0 + a = a.
   Proof. lia. Qed.
 
-  Lemma mempty_app_r : forall (a : A), a + 0 = a.
+  Lemma mempty_app_r : forall (a : nat), a + 0 = a.
   Proof. lia. Qed.
 
-  Lemma mappend_assoc : forall (x y z : A), x + y + z = x + (y + z).
+  Lemma mappend_assoc : forall (x y z : nat), x + y + z = x + (y + z).
   Proof. lia. Qed.
-End AdditionMonoidSpec.
+End AddMonoidSpec.
+
+Module AddMonoidFactory := MonoidFactory AddMonoidSpec.
+Definition AddMonoid : Monoid nat :=
+  AddMonoidFactory.MonoidInstance.
+(**[]*)
+
+(** Multiplication of Naturals. *)
+Module MulMonoidSpec <: MonoidSpec.
+  Definition A : Type := nat.
+
+  Definition mempty : nat := 1.
+
+  Definition mappend : nat -> nat -> nat := mul.
+
+  Lemma mempty_app_l : forall (a : nat), 1 * a = a.
+  Proof. lia. Qed.
+
+  Lemma mempty_app_r : forall (a : nat), a * 1 = a.
+  Proof. lia. Qed.
+
+  Lemma mappend_assoc : forall (x y z : nat),
+      x * y * z = x * (y * z).
+  Proof. lia. Qed.
+End MulMonoidSpec.
+
+Module MulMonoidFactory := MonoidFactory MulMonoidSpec.
+Definition MulMonoid : Monoid nat :=
+  MulMonoidFactory.MonoidInstance.
+(**[]*)
+
+(** * Parameterized Monoids *)
+
+Module Type ParamMonoidSpec.
+  Parameter M : Type -> Type.
+  Section Spec.
+    Context {A : Type}.
+    Parameter mempty : M A.
+    Parameter mappend : M A -> M A -> M A.
+    Parameter mempty_app_l : forall (m : M A), mappend mempty m = m.
+    Parameter mempty_app_r : forall (m : M A), mappend m mempty = m.
+    Parameter mappend_assoc : forall (x y z : M A),
+      mappend (mappend x y) z = mappend x (mappend y z).
+  End Spec.
+End ParamMonoidSpec.
+
+Module ParamMonoidFactory (MS : ParamMonoidSpec).
+  Instance ParamMonoidInstance (A : Type) : Monoid (MS.M A) :=
+    { mempty := @MS.mempty A;
+      mappend := @MS.mappend A;
+      mempty_app_l := @MS.mempty_app_l A;
+      mempty_app_r := @MS.mempty_app_r A;
+      mappend_assoc := @MS.mappend_assoc A }.
+End ParamMonoidFactory.
+
+(** Lists. *)
+Module ListMonoidSpec <: ParamMonoidSpec.
+  Import ListNotations.
+
+  Definition M : Type -> Type := list.
+
+  Section Spec.
+    Context {A : Type}.
+
+    Definition mempty : list A := [].
+
+    Definition mappend : list A -> list A -> list A := @app A.
+
+    Lemma mempty_app_l : forall (m : list A), [] ++ m = m.
+    Proof. reflexivity. Qed.
+
+    Lemma mempty_app_r : forall (m : list A), m ++ [] = m.
+    Proof. intros. apply app_nil_r. Qed.
+
+    Lemma mappend_assoc : forall (x y z : list A),
+     (x ++ y) ++ z = x ++ (y ++ z).
+    Proof. intros. rewrite app_assoc. reflexivity. Qed.
+  End Spec.
+End ListMonoidSpec.
+
+Module ListMonoidFactory := ParamMonoidFactory ListMonoidSpec.
+Definition ListMonoid (A : Type) : Monoid (list A) :=
+  ListMonoidFactory.ParamMonoidInstance A.
+
+(** Function Composition. *)
+Module ArrowMonoidSpec <: ParamMonoidSpec.
+  Definition M : Type -> Type := fun A => A -> A.
+
+  Section Spec.
+    Context {A : Type}.
+
+    Definition mempty : A -> A := id.
+
+    Definition mappend : (A -> A) -> (A -> A) -> (A -> A) := compose.
+
+    Lemma mempty_app_l : forall (m : A -> A), id ∘ m = m.
+    Proof. intros. reflexivity. Qed.
+
+    Lemma mempty_app_r : forall (m : A -> A), m ∘ id = m.
+    Proof. intros. reflexivity. Qed.
+
+    Lemma mappend_assoc : forall (x y z : A -> A),
+      x ∘ y ∘ z = x ∘ (y ∘ z).
+    Proof. intros. reflexivity. Qed.
+  End Spec.
+End ArrowMonoidSpec.
+
+Module ArrowMonoidFactory := ParamMonoidFactory ArrowMonoidSpec.
+Definition ArrowMonoid (A : Type) : Monoid (A -> A) :=
+  ArrowMonoidFactory.ParamMonoidInstance A.
+(**[]*)
